semantics/proofs/evalPropsScript.sml
@@ -132,5 +132,50 @@ val same_tid_sym = Q.store_thm ("same_tid_sym",
  rw [same_tid_def] >>
  metis_tac []);
 
+val build_tdefs_cons = Q.store_thm ("build_tdefs_cons",
+`(!tvs tn ctors tds mn.
+  build_tdefs mn ((tvs,tn,ctors)::tds) =
+    (MAP (\(conN,ts). (conN, LENGTH ts, TypeId (mk_id mn tn)))
+        ctors) ++ build_tdefs mn tds) ∧
+ (!mn. build_tdefs mn [] = [])`,
+rw [build_tdefs_def]);
+
+val check_ctor_foldr_flat_map = Q.prove (
+`!c. (FOLDR
+         (λ(tvs,tn,condefs) x2.
+            FOLDR (λ(n,ts) x2. n::x2) x2 condefs) [] c)
+    =
+    FLAT (MAP (\(tvs,tn,condefs). (MAP (λ(n,ts). n)) condefs) c)`,
+induct_on `c` >>
+rw [LET_THM] >>
+PairCases_on `h` >>
+fs [LET_THM] >>
+pop_assum (fn _ => all_tac) >>
+induct_on `h2` >>
+rw [] >>
+PairCases_on `h` >>
+rw []);
+
+val check_dup_ctors_thm = Q.store_thm ("check_dup_ctors_thm",
+`!tds.
+  check_dup_ctors tds =
+    ALL_DISTINCT (FLAT (MAP (\(tvs,tn,condefs). (MAP (λ(n,ts). n)) condefs) tds))`,
+metis_tac [check_dup_ctors_def,check_ctor_foldr_flat_map]);
+
+val check_dup_ctors_cons = Q.store_thm ("check_dup_ctors_cons",
+`!tvs ts ctors tds.
+  check_dup_ctors ((tvs,ts,ctors)::tds)
+  ⇒
+  check_dup_ctors tds`,
+induct_on `tds` >>
+rw [check_dup_ctors_def, LET_THM, RES_FORALL] >>
+PairCases_on `h` >>
+fs [] >>
+pop_assum MP_TAC >>
+pop_assum (fn _ => all_tac) >>
+induct_on `ctors` >>
+rw [] >>
+PairCases_on `h` >>
+fs []);
 
 val _ = export_theory ();
